@prefix : <http://www.semanticweb.org/owl/owlapi/turtle#> .
@prefix sp: <http://spinrdf.org/sp#> .
@prefix ns1: <http://web.resource.org/cc/> .
@prefix owl: <http://www.w3.org/2002/07/owl#> .
@prefix rdf: <http://www.w3.org/1999/02/22-rdf-syntax-ns#> .
@prefix spl: <http://spinrdf.org/spl#> .
@prefix xml: <http://www.w3.org/XML/1998/namespace> .
@prefix xsd: <http://www.w3.org/2001/XMLSchema#> .
@prefix prov: <http://www.w3.org/ns/prov#> .
@prefix rdfs: <http://www.w3.org/2000/01/rdf-schema#> .
@prefix spin: <http://spinrdf.org/spin#> .
@prefix dcterm: <http://purl.org/dc/terms/> .
@prefix p-plan: <http://purl.org/net/p-plan#> .
@prefix SC-PROV-0: <http://example.org/SC-PROV-0.1#> .
@base <https://w3id.org/abdn/socialcomp/sc-prov> .

<https://w3id.org/abdn/socialcomp/sc-prov> rdf:type owl:Ontology ;
                                           
                                           rdfs:label "SC-PROV-O: An ontology for describing provenance of social computation"@en ;
                                           
                                           owl:versionInfo "0.0.1"^^xsd:string ;
                                           
                                           dcterm:rights "Copyright Â© 2015 Milan Markovic" ;
                                           
                                           ns1:license <http://creativecommons.org/licenses/by-sa/3.0/> ;
                                           
                                           owl:imports p-plan: ,
                                                       <http://www.w3.org/ns/prov-o-20130430> .


#################################################################
#
#    Object Properties
#
#################################################################


###  http://example.org/SC-PROV-0.1#correspondsToActor

SC-PROV-0:correspondsToActor rdf:type owl:FunctionalProperty ,
                                      owl:ObjectProperty ;
                             
                             rdfs:label "correspondsToActor"^^xsd:string ;
                             
                             rdfs:comment "A relation that links a prov:Agent to its expected description captured by sc-prov-o:SocialActorSpec."^^xsd:string ;
                             
                             rdfs:range SC-PROV-0:SocialActorSpec ;
                             
                             rdfs:domain prov:Agent .



###  http://example.org/SC-PROV-0.1#hadCondition

SC-PROV-0:hadCondition rdf:type owl:FunctionalProperty ,
                                owl:ObjectProperty ;
                       
                       rdfs:label "hadCondition"^^xsd:string ;
                       
                       rdfs:comment "A relation that links a specific sc-prov-o:evaluationContext to the sc-prov-o:Condition for which the evaluation was sought for."^^xsd:string ;
                       
                       rdfs:range SC-PROV-0:Condition ;
                       
                       rdfs:domain SC-PROV-0:EvaluationContext .



###  http://example.org/SC-PROV-0.1#hadEvaluationSubject

SC-PROV-0:hadEvaluationSubject rdf:type owl:FunctionalProperty ,
                                        owl:ObjectProperty ;
                               
                               rdfs:label "hadActivity"^^xsd:string ;
                               
                               rdfs:comment """A relation describing that a particular p-plan:Activity captured as
part of the sc-prov-o:EvaluationContext is the activity for which the condition was evaluated."""^^xsd:string ;
                               
                               rdfs:domain SC-PROV-0:EvaluationContext ;
                               
                               rdfs:range p-plan:Activity .



###  http://example.org/SC-PROV-0.1#hadParameterCollection

SC-PROV-0:hadParameterCollection rdf:type owl:ObjectProperty ;
                                 
                                 rdfs:label "had Parameter Collection" ;
                                 
                                 rdfs:comment "A relation that is used to associate an sc-prov:ParameterCollection with an sc-prov:EvaluationContext" .



###  http://example.org/SC-PROV-0.1#hadResult

SC-PROV-0:hadResult rdf:type owl:FunctionalProperty ,
                             owl:ObjectProperty ;
                    
                    rdfs:label "hadResult"^^xsd:string ;
                    
                    rdfs:comment "A relation describing that a particular p-plan:Entity represents the evaluation result of specific condition applicable to the state of the world described by the sc- prov-o:EvaluationContext."^^xsd:string ;
                    
                    rdfs:domain SC-PROV-0:EvaluationContext ;
                    
                    rdfs:range p-plan:Entity .



###  http://example.org/SC-PROV-0.1#hasIncentive

SC-PROV-0:hasIncentive rdf:type owl:ObjectProperty ;
                       
                       rdfs:label "hasIncentive"@en ;
                       
                       rdfs:comment "placeholder"@en ;
                       
                       rdfs:range SC-PROV-0:Incentive ;
                       
                       rdfs:domain p-plan:Step .



###  http://example.org/SC-PROV-0.1#hasParameter

SC-PROV-0:hasParameter rdf:type owl:ObjectProperty ;
                       
                       rdfs:label "hasParameter"@en ;
                       
                       rdfs:comment """sc-prov:hasParameter is a relation defining that a p-plan:Variable provides a
parameter value for the sc-prov:Condition."""@en ;
                       
                       rdfs:domain SC-PROV-0:Condition ;
                       
                       rdfs:range p-plan:Variable .



###  http://example.org/SC-PROV-0.1#hasRoleSpec

SC-PROV-0:hasRoleSpec rdf:type owl:FunctionalProperty ,
                               owl:ObjectProperty ;
                      
                      rdfs:label "hasRoleSpec"@en ;
                      
                      rdfs:comment "A relation that links an instance of sc-prov-o:Purpose with a single specifica- tion of the assigned sc-prov-o: RoleSpec."@en ;
                      
                      rdfs:domain SC-PROV-0:Purpose ;
                      
                      rdfs:range SC-PROV-0:RoleSpec .



###  http://example.org/SC-PROV-0.1#isConditionOfPlan

SC-PROV-0:isConditionOfPlan rdf:type owl:ObjectProperty ;
                            
                            rdfs:label "isConditionOfPlan"@en ;
                            
                            rdfs:comment "Links an instance of an sc-prov-o:Condition to a specific instance of a p-plan:Plan"@en ;
                            
                            rdfs:domain SC-PROV-0:Condition ;
                            
                            rdfs:range prov:Plan .



###  http://example.org/SC-PROV-0.1#isImposedOn

SC-PROV-0:isImposedOn rdf:type owl:ObjectProperty ;
                      
                      rdfs:label "isImposedOn"@en ;
                      
                      rdfs:comment "sc-prov:isImposedOn is a relation defining that an sc-prov:Condition is defined for a p-plan:Step."@en ;
                      
                      rdfs:domain SC-PROV-0:Condition ;
                      
                      rdfs:range p-plan:Step .



###  http://example.org/SC-PROV-0.1#isPurposeInPlan

SC-PROV-0:isPurposeInPlan rdf:type owl:ObjectProperty ;
                          
                          rdfs:label "isPurposeInPlan"@en ;
                          
                          rdfs:comment "Links an instance of a sc-prov-o:Purpose to a specific instance of a p-plan:Plan"@en ;
                          
                          rdfs:domain SC-PROV-0:Purpose ;
                          
                          rdfs:subPropertyOf owl:topObjectProperty ;
                          
                          rdfs:range prov:Plan .



###  http://example.org/SC-PROV-0.1#performs

SC-PROV-0:performs rdf:type owl:ObjectProperty ;
                   
                   rdfs:label "performs"@en ;
                   
                   rdfs:comment "sc-prov:performs is a relation defining that an sc-prov:socialActor defines a description of an agent that will bear some responsibility for the activity described by p-plan:Step."@en ;
                   
                   rdfs:domain SC-PROV-0:SocialActorSpec ;
                   
                   owl:propertyDisjointWith SC-PROV-0:requests ;
                   
                   rdfs:range p-plan:Step .



###  http://example.org/SC-PROV-0.1#qualifiedAction

SC-PROV-0:qualifiedAction rdf:type owl:ObjectProperty ;
                          
                          rdfs:label "qualifiedAction"@en ;
                          
                          rdfs:comment """A relation that links an sc-prov-o: SocialActorSpec to the scope of the expected
activity performed by agents that correspond to such sc-prov-o: SocialActorSpec."""@en ;
                          
                          rdfs:range SC-PROV-0:Action ;
                          
                          rdfs:domain SC-PROV-0:SocialActorSpec ;
                          
                          rdfs:subPropertyOf SC-PROV-0:qualifiedPurpose .



###  http://example.org/SC-PROV-0.1#qualifiedImposition

SC-PROV-0:qualifiedImposition rdf:type owl:ObjectProperty ;
                              
                              rdfs:label "qualifiedImposition"@en ;
                              
                              rdfs:comment """A relation that links an sc-prov-o: Condition to an sc-prov-o: Imposition which
describes the subjection of a p-plan:Step to the constraints described by the sc-prov:Condition."""@en ;
                              
                              rdfs:domain SC-PROV-0:Condition ;
                              
                              rdfs:range SC-PROV-0:Imposition ;
                              
                              rdfs:subPropertyOf SC-PROV-0:qualifiedPurpose .



###  http://example.org/SC-PROV-0.1#qualifiedInput

SC-PROV-0:qualifiedInput rdf:type owl:ObjectProperty ;
                         
                         rdfs:label "qualifiedInput"@en ;
                         
                         rdfs:comment "A relation that links a p-plan: Variable to the description of the specification context in which a variable is expected to be taken as an input for a step (sc-prov-o: Input)."@en ;
                         
                         rdfs:range SC-PROV-0:Input ;
                         
                         rdfs:subPropertyOf SC-PROV-0:qualifiedPurpose ;
                         
                         rdfs:domain p-plan:Variable .



###  http://example.org/SC-PROV-0.1#qualifiedOutput

SC-PROV-0:qualifiedOutput rdf:type owl:ObjectProperty ;
                          
                          rdfs:label "qualifiedOutput"@en ;
                          
                          rdfs:comment "A relation that links a p-plan: Variable to the description of the specification context in which a variable is expected to be produced as an output of a step (sc-prov-o: Output)."@en ;
                          
                          rdfs:range SC-PROV-0:Output ;
                          
                          rdfs:subPropertyOf SC-PROV-0:qualifiedPurpose ;
                          
                          rdfs:domain p-plan:Variable .



###  http://example.org/SC-PROV-0.1#qualifiedPurpose

SC-PROV-0:qualifiedPurpose rdf:type owl:ObjectProperty ;
                           
                           rdfs:label "qualifiedPurpose"@en ;
                           
                           rdfs:comment """A relation that links a p-plan:Variable or an sc-prov:Condition with the descrip-
tion of their expected scope of influence on a p-plan:Step."""@en ;
                           
                           rdfs:range SC-PROV-0:Purpose ;
                           
                           rdfs:domain [ rdf:type owl:Class ;
                                         owl:unionOf ( SC-PROV-0:Condition
                                                       p-plan:Variable
                                                     )
                                       ] .



###  http://example.org/SC-PROV-0.1#requests

SC-PROV-0:requests rdf:type owl:ObjectProperty ;
                   
                   rdfs:label "requests"@en ;
                   
                   rdfs:comment "sc-prov:requests is a relation defining that a prov:Agent corresponding to the sc-prov:socialActor description is responsible for existence of the particular p-plan:Step."@en ;
                   
                   rdfs:domain SC-PROV-0:SocialActorSpec ;
                   
                   rdfs:range p-plan:Step .



###  http://example.org/SC-PROV-0.1#target

SC-PROV-0:target rdf:type owl:FunctionalProperty ,
                          owl:ObjectProperty ;
                 
                 rdfs:label "target"@en ;
                 
                 rdfs:comment "A relation that links an sc-prov-o:Purpose with the subject of its influence, i.e. a p-plan:Step."@en ;
                 
                 rdfs:range p-plan:Step ;
                 
                 rdfs:domain [ rdf:type owl:Class ;
                               owl:unionOf ( SC-PROV-0:Condition
                                             p-plan:Variable
                                           )
                             ] .





#################################################################
#
#    Classes
#
#################################################################


###  http://example.org/SC-PROV-0.1#Action

SC-PROV-0:Action rdf:type owl:Class ;
                 
                 rdfs:label "Action"@en ;
                 
                 rdfs:subClassOf SC-PROV-0:Purpose ;
                 
                 rdfs:comment "Action is the scope of the expected activity performed by agents that correspond to sc-prov:SocialActorSpec."@en .



###  http://example.org/SC-PROV-0.1#Condition

SC-PROV-0:Condition rdf:type owl:Class ;
                    
                    rdfs:label "Condition"@en ;
                    
                    rdfs:subClassOf owl:Thing ;
                    
                    rdfs:comment "An sc-prov:Condition defines a state of the world described by a logical state- ment that is used to define a desired state of a particular aspect of a successful step."@en .



###  http://example.org/SC-PROV-0.1#EvaluationContext

SC-PROV-0:EvaluationContext rdf:type owl:Class ;
                            
                            rdfs:label "Evaluation Context"@en ;
                            
                            rdfs:subClassOf owl:Thing ;
                            
                            rdfs:comment "A concept used to connect the evaluation result of a particular sc-prov:Condition (C1) with a single executed p-plan:Activity corresponding to the step associated with C1."@en .



###  http://example.org/SC-PROV-0.1#Imposition

SC-PROV-0:Imposition rdf:type owl:Class ;
                     
                     rdfs:label "Imposition"@en ;
                     
                     rdfs:subClassOf SC-PROV-0:Purpose ;
                     
                     rdfs:comment "Imposition is the subjection of p-plan:Step to the constraints described by sc- prov:Condition."@en .



###  http://example.org/SC-PROV-0.1#Incentive

SC-PROV-0:Incentive rdf:type owl:Class ;
                    
                    rdfs:label "Incentive"@en ;
                    
                    rdfs:subClassOf p-plan:Variable ;
                    
                    owl:disjointWith SC-PROV-0:SocialActorSpec ;
                    
                    rdfs:comment "Incentive is a kind of p-plan:Variable and represents a thing (e.g. monetary value, increased knowledge, etc.) that would be realised by a worker following successful completion of a task."@en .



###  http://example.org/SC-PROV-0.1#Input

SC-PROV-0:Input rdf:type owl:Class ;
                
                rdfs:label "Input"@en ;
                
                rdfs:subClassOf SC-PROV-0:Purpose ;
                
                rdfs:comment "Input describes a specification context in which a p-plan:Variable is expected to be taken as an input for a p-plan:Step."@en .



###  http://example.org/SC-PROV-0.1#Output

SC-PROV-0:Output rdf:type owl:Class ;
                 
                 rdfs:label "Output"@en ;
                 
                 rdfs:subClassOf SC-PROV-0:Purpose ;
                 
                 rdfs:comment """Output describes a specification context in which a p-plan:Variable is expected
to be produced as an output of a p-plan:Step."""@en .



###  http://example.org/SC-PROV-0.1#ParameterCollection

SC-PROV-0:ParameterCollection rdf:type owl:Class ;
                              
                              rdfs:label "Parameter Collection"@en ;
                              
                              rdfs:subClassOf prov:Collection ;
                              
                              rdfs:comment """A kind of prov:Collection which is used to encapsulate the in-
stances of prov:Entity that were used as parameters to evaluate a particular sc-prov:Condition."""@en .



###  http://example.org/SC-PROV-0.1#Purpose

SC-PROV-0:Purpose rdf:type owl:Class ;
                  
                  rdfs:label "Purpose"@en ;
                  
                  rdfs:subClassOf owl:Thing ;
                  
                  rdfs:comment "Purpose is the expected scope of influence of a p-plan:Variable or an sc- prov:Condition on a p-plan:Step."@en .



###  http://example.org/SC-PROV-0.1#RoleSpec

SC-PROV-0:RoleSpec rdf:type owl:Class ;
                   
                   rdfs:label "Role Specification"@en ;
                   
                   rdfs:subClassOf owl:Thing ;
                   
                   rdfs:comment "A role specification is the function of a variable, a social actor, or a condition in the context of a particular step."@en .



###  http://example.org/SC-PROV-0.1#SocialActorSpec

SC-PROV-0:SocialActorSpec rdf:type owl:Class ;
                          
                          rdfs:label "Social Actor Specification"@en ;
                          
                          rdfs:subClassOf p-plan:Variable ;
                          
                          rdfs:comment "An sc-prov:SocialActor is a kind of p-plan:Variable and represents a desired specification of an agent who should be associated with a p-plan:Step in order to perform a non- administrative function in a social computation process."@en .





#################################################################
#
#    General axioms
#
#################################################################


[ rdf:type owl:AllDisjointClasses ;
  owl:members ( SC-PROV-0:Action
                SC-PROV-0:Imposition
                SC-PROV-0:Input
                SC-PROV-0:Output
              )
] .
[ rdf:type owl:AllDisjointClasses ;
  owl:members ( SC-PROV-0:Condition
                p-plan:Step
                p-plan:Variable
              )
] .




###  Generated by the OWL API (version 3.5.1) http://owlapi.sourceforge.net

